Clean up and improve Reflection.Relations

src/Reflection/Relations.v
@@ -6,6 +6,8 @@ Require Import Crypto.Util.Tactics.
 Require Import Crypto.Util.Prod.
 Require Import Crypto.Util.Sigma.
 
+Local Coercion is_true : bool >-> Sortclass.
+
 Local Open Scope ctype_scope.
 Section language.
   Context {base_type_code : Type}.
@@ -13,240 +15,252 @@ Section language.
   Local Notation flat_type := (flat_type base_type_code).
   Local Notation type := (type base_type_code).
 
-  Section type.
-    Context (interp_flat_type : flat_type -> Type)
-            (R : forall t, interp_flat_type t -> interp_flat_type t -> Prop).
-    Local Notation interp_type_gen := (interp_type_gen interp_flat_type).
-    Fixpoint interp_type_gen_rel_pointwise (t : type)
-      : interp_type_gen t -> interp_type_gen t -> Prop :=
-      match t with
-      | Tflat t => R t
-      | Arrow _ y => fun f g => forall x, interp_type_gen_rel_pointwise y (f x) (g x)
-      end.
-    Global Instance interp_type_gen_rel_pointwise_Reflexive {H : forall t, Reflexive (R t)}
-      : forall t, Reflexive (interp_type_gen_rel_pointwise t).
-    Proof. induction t; repeat intro; reflexivity. Qed.
-    Global Instance interp_type_gen_rel_pointwise_Symmetric {H : forall t, Symmetric (R t)}
-      : forall t, Symmetric (interp_type_gen_rel_pointwise t).
-    Proof. induction t; simpl; repeat intro; symmetry; eauto. Qed.
-    Global Instance interp_type_gen_rel_pointwise_Transitive {H : forall t, Transitive (R t)}
-      : forall t, Transitive (interp_type_gen_rel_pointwise t).
-    Proof. induction t; simpl; repeat intro; etransitivity; eauto. Qed.
-  End type.
-
-  Section flat_type0.
-    Context {interp_base_type : base_type_code -> Type}
-            (R : forall t, interp_base_type t -> Prop).
-    Local Notation interp_flat_type := (interp_flat_type interp_base_type).
-    Fixpoint interp_flat_type_rel_pointwise0 (t : flat_type)
-      : interp_flat_type t -> Prop :=
-      match t with
-      | Tbase t => R t
-      | Unit => fun _ => True
-      | Prod _ _ => fun x => interp_flat_type_rel_pointwise0 _ (fst x)
-                             /\ interp_flat_type_rel_pointwise0 _ (snd x)
-      end.
-  End flat_type0.
+  Local Ltac rel_relb_t :=
+    repeat first [ progress simpl in *
+                 | reflexivity
+                 | intuition congruence
+                 | setoid_rewrite Bool.andb_true_iff
+                 | intro
+                 | rewrite_hyp <- !* ].
 
   Section flat_type.
-    Context {interp_base_type : base_type_code -> Type}
-            (R : forall t, interp_base_type t -> interp_base_type t -> Prop).
-    Local Notation interp_flat_type := (interp_flat_type interp_base_type).
-    Fixpoint interp_flat_type_rel_pointwise (t : flat_type)
-      : interp_flat_type t -> interp_flat_type t -> Prop :=
-      match t with
-      | Tbase t => R t
-      | Unit => fun _ _ => True
-      | Prod _ _ => fun x y => interp_flat_type_rel_pointwise _ (fst x) (fst y)
-                               /\ interp_flat_type_rel_pointwise _ (snd x) (snd y)
-      end.
-    Definition interp_type_rel_pointwise
-      := interp_type_gen_rel_pointwise _ interp_flat_type_rel_pointwise.
+    Context {interp_base_type1 interp_base_type2 : base_type_code -> Type}.
+    Local Notation interp_flat_type1 := (interp_flat_type interp_base_type1).
+    Local Notation interp_flat_type2 := (interp_flat_type interp_base_type2).
+
+    Section gen_Prop.
+      Context (P : Type)
+              (and : P -> P -> P)
+              (True : P)
+              (False : P).
+      Section pointwise1.
+        Context (R : forall t, interp_base_type1 t -> P).
+        Fixpoint interp_flat_type_rel_pointwise1_gen_Prop (t : flat_type)
+          : interp_flat_type1 t -> P :=
+          match t with
+          | Tbase t => R t
+          | Unit => fun _ => True
+          | Prod _ _ => fun x => and (interp_flat_type_rel_pointwise1_gen_Prop _ (fst x))
+                                     (interp_flat_type_rel_pointwise1_gen_Prop _ (snd x))
+          end.
+      End pointwise1.
+      Section pointwise2.
+        Context (R : forall t, interp_base_type1 t -> interp_base_type2 t -> P).
+        Fixpoint interp_flat_type_rel_pointwise_gen_Prop (t : flat_type)
+          : interp_flat_type1 t -> interp_flat_type2 t -> P :=
+          match t with
+          | Tbase t => R t
+          | Unit => fun _ _ => True
+          | Prod _ _ => fun x y => and (interp_flat_type_rel_pointwise_gen_Prop _ (fst x) (fst y))
+                                       (interp_flat_type_rel_pointwise_gen_Prop _ (snd x) (snd y))
+          end.
+      End pointwise2.
+      Section pointwise2_hetero.
+        Context (R : forall t1 t2, interp_base_type1 t1 -> interp_base_type2 t2 -> P).
+        Fixpoint interp_flat_type_rel_pointwise_hetero_gen_Prop (t1 t2 : flat_type)
+          : interp_flat_type1 t1 -> interp_flat_type2 t2 -> P
+          := match t1, t2 with
+             | Tbase t1, Tbase t2 => R t1 t2
+             | Unit, Unit => fun _ _ => True
+             | Prod x1 y1, Prod x2 y2
+               => fun a b => and (interp_flat_type_rel_pointwise_hetero_gen_Prop x1 x2 (fst a) (fst b))
+                                 (interp_flat_type_rel_pointwise_hetero_gen_Prop y1 y2 (snd a) (snd b))
+             | Tbase _, _
+             | Unit, _
+             | Prod _ _, _
+               => fun _ _ => False
+             end.
+      End pointwise2_hetero.
+    End gen_Prop.
+
+    Definition interp_flat_type_relb_pointwise1
+      := @interp_flat_type_rel_pointwise1_gen_Prop bool andb true.
+    Global Arguments interp_flat_type_relb_pointwise1 _ !_ _ / .
+    Definition interp_flat_type_rel_pointwise1
+      := @interp_flat_type_rel_pointwise1_gen_Prop Prop and True.
+    Global Arguments interp_flat_type_rel_pointwise1 _ !_ _ / .
+    Lemma interp_flat_type_rel_pointwise1_iff_relb {R} t x
+      : interp_flat_type_relb_pointwise1 R t x <-> interp_flat_type_rel_pointwise1 R t x.
+    Proof. clear; induction t; rel_relb_t. Qed.
+    Definition interp_flat_type_relb_pointwise
+      := @interp_flat_type_rel_pointwise_gen_Prop bool andb true.
+    Global Arguments interp_flat_type_relb_pointwise _ !_ _ _ / .
+    Definition interp_flat_type_rel_pointwise
+      := @interp_flat_type_rel_pointwise_gen_Prop Prop and True.
+    Global Arguments interp_flat_type_rel_pointwise _ !_ _ _ / .
+    Lemma interp_flat_type_rel_pointwise_iff_relb {R} t x y
+      : interp_flat_type_relb_pointwise R t x y <-> interp_flat_type_rel_pointwise R t x y.
+    Proof. clear; induction t; rel_relb_t. Qed.
+    Definition interp_flat_type_relb_pointwise_hetero
+      := @interp_flat_type_rel_pointwise_hetero_gen_Prop bool andb true false.
+    Global Arguments interp_flat_type_relb_pointwise_hetero _ !_ !_ _ _ / .
+    Definition interp_flat_type_rel_pointwise_hetero
+      := @interp_flat_type_rel_pointwise_hetero_gen_Prop Prop and True False.
+    Global Arguments interp_flat_type_rel_pointwise_hetero _ !_ !_ _ _ / .
+    Lemma interp_flat_type_rel_pointwise_hetero_iff_relb {R} t1 t2 x y
+      : interp_flat_type_relb_pointwise_hetero R t1 t2 x y <-> interp_flat_type_rel_pointwise_hetero R t1 t2 x y.
+    Proof. clear; revert dependent t2; induction t1, t2; rel_relb_t. Qed.
+
+    Lemma interp_flat_type_rel_pointwise_hetero_iff {R t} x y
+      : interp_flat_type_rel_pointwise (fun t => R t t) t x y
+        <-> interp_flat_type_rel_pointwise_hetero R t t x y.
+    Proof. induction t; simpl; rewrite_hyp ?*; reflexivity. Qed.
   End flat_type.
 
-  Section rel_pointwise2.
-    Section type.
+  Section type.
+    Section hetero.
+      Context (interp_src1 interp_src2 : base_type_code -> Type)
+              (interp_dst1 interp_dst2 : flat_type -> Type).
+      Section hetero.
+        Context (Rsrc : forall t, interp_src1 t -> interp_src2 t -> Prop)
+                (Rdst : forall t, interp_dst1 t -> interp_dst2 t -> Prop).
+
+        Fixpoint interp_type_gen_rel_pointwise_hetero (t : type)
+          : interp_type_gen_hetero interp_src1 interp_dst1 t
+            -> interp_type_gen_hetero interp_src2 interp_dst2 t
+            -> Prop
+          := match t with
+             | Tflat t => Rdst t
+             | Arrow src dst => @respectful_hetero _ _ _ _ (Rsrc src) (fun _ _ => interp_type_gen_rel_pointwise_hetero dst)
+             end.
+        Global Arguments interp_type_gen_rel_pointwise_hetero _ _ _ / .
+      End hetero.
       Section hetero_hetero.
-        Context (interp_src1 interp_src2 : base_type_code -> Type)
-                (interp_dst1 interp_dst2 : flat_type -> Type)
-                (Rsrc : forall t1 t2, interp_src1 t1 -> interp_src2 t2 -> Prop)
+        Context (Rsrc : forall t1 t2, interp_src1 t1 -> interp_src2 t2 -> Prop)
                 (Rdst : forall t1 t2, interp_dst1 t1 -> interp_dst2 t2 -> Prop).
 
-        Fixpoint interp_type_gen_rel_pointwise2_hetero_hetero (t1 t2 : type)
+        Fixpoint interp_type_gen_rel_pointwise_hetero_hetero (t1 t2 : type)
           : interp_type_gen_hetero interp_src1 interp_dst1 t1
             -> interp_type_gen_hetero interp_src2 interp_dst2 t2
             -> Prop
           := match t1, t2 with
              | Tflat t1, Tflat t2 => Rdst t1 t2
              | Arrow src1 dst1, Arrow src2 dst2
-               => @respectful_hetero _ _ _ _ (Rsrc src1 src2) (fun _ _ => interp_type_gen_rel_pointwise2_hetero_hetero dst1 dst2)
+               => @respectful_hetero _ _ _ _ (Rsrc src1 src2) (fun _ _ => interp_type_gen_rel_pointwise_hetero_hetero dst1 dst2)
              | Tflat _, _
              | Arrow _ _, _
                => fun _ _ => False
              end.
-        Global Arguments interp_type_gen_rel_pointwise2_hetero_hetero _ _ _ _ / .
+        Global Arguments interp_type_gen_rel_pointwise_hetero_hetero _ _ _ _ / .
       End hetero_hetero.
-      Section hetero.
-        Context (interp_src1 interp_src2 : base_type_code -> Type)
-                (interp_dst1 interp_dst2 : flat_type -> Type)
-                (Rsrc : forall t, interp_src1 t -> interp_src2 t -> Prop)
-                (Rdst : forall t, interp_dst1 t -> interp_dst2 t -> Prop).
+    End hetero.
 
-        Fixpoint interp_type_gen_rel_pointwise2_hetero (t : type)
-          : interp_type_gen_hetero interp_src1 interp_dst1 t
-            -> interp_type_gen_hetero interp_src2 interp_dst2 t
-            -> Prop
-          := match t with
-             | Tflat t => Rdst t
-             | Arrow src dst => @respectful_hetero _ _ _ _ (Rsrc src) (fun _ _ => interp_type_gen_rel_pointwise2_hetero dst)
-             end.
-        Global Arguments interp_type_gen_rel_pointwise2_hetero _ _ _ / .
-      End hetero.
-      Section homogenous.
-        Context (interp_flat_type1 interp_flat_type2 : flat_type -> Type)
-                (R : forall t, interp_flat_type1 t -> interp_flat_type2 t -> Prop).
+    Section partially_hetero.
+      Context (interp_flat_type1 interp_flat_type2 : flat_type -> Type)
+              (R : forall t, interp_flat_type1 t -> interp_flat_type2 t -> Prop).
 
-        Let Tbase := (@Tbase base_type_code).
-        Local Coercion Tbase : base_type_code >-> flat_type.
+      Definition interp_type_gen_rel_pointwise2
+        : forall t,
+          interp_type_gen interp_flat_type1 t
+          -> interp_type_gen interp_flat_type2 t
+          -> Prop
+        := interp_type_gen_rel_pointwise_hetero
+             (fun t => interp_flat_type1 (Tbase t)) (fun t => interp_flat_type2 (Tbase t))
+             interp_flat_type1 interp_flat_type2
+             (fun t => R (Tbase t)) R.
+      Global Arguments interp_type_gen_rel_pointwise2 _ _ _ / .
+    End partially_hetero.
 
-        Definition interp_type_gen_rel_pointwise2
-          : forall t,
-            interp_type_gen interp_flat_type1 t
-            -> interp_type_gen interp_flat_type2 t
-            -> Prop
-          := interp_type_gen_rel_pointwise2_hetero interp_flat_type1 interp_flat_type2
-                                                   interp_flat_type1 interp_flat_type2
-                                                   R R.
-      End homogenous.
-      Global Arguments interp_type_gen_rel_pointwise2 _ _ _ _ _ _ / .
-    End type.
-    Section flat_type.
+    Section homogenous.
+      Context (interp_flat_type : flat_type -> Type)
+              (R : forall t, interp_flat_type t -> interp_flat_type t -> Prop).
+      Local Notation interp_type_gen := (interp_type_gen interp_flat_type).
+      Fixpoint interp_type_gen_rel_pointwise (t : type)
+        : interp_type_gen t -> interp_type_gen t -> Prop :=
+        match t with
+        | Tflat t => R t
+        | Arrow _ y => fun f g => forall x, interp_type_gen_rel_pointwise y (f x) (g x)
+        end.
+      Global Instance interp_type_gen_rel_pointwise_Reflexive {H : forall t, Reflexive (R t)}
+        : forall t, Reflexive (interp_type_gen_rel_pointwise t).
+      Proof. induction t; repeat intro; reflexivity. Qed.
+      Global Instance interp_type_gen_rel_pointwise_Symmetric {H : forall t, Symmetric (R t)}
+        : forall t, Symmetric (interp_type_gen_rel_pointwise t).
+      Proof. induction t; simpl; repeat intro; symmetry; eauto. Qed.
+      Global Instance interp_type_gen_rel_pointwise_Transitive {H : forall t, Transitive (R t)}
+        : forall t, Transitive (interp_type_gen_rel_pointwise t).
+      Proof. induction t; simpl; repeat intro; etransitivity; eauto. Qed.
+    End homogenous.
+  End type.
+
+  Section specialized_type.
+    Section hetero.
       Context (interp_base_type1 interp_base_type2 : base_type_code -> Type).
-      Section gen_prop.
-        Context (P : Type)
-                (and : P -> P -> P)
-                (True : P)
-                (False : P).
-        Section hetero.
-          Context (R : forall t1 t2, interp_base_type1 t1 -> interp_base_type2 t2 -> P).
-
-          Fixpoint interp_flat_type_rel_pointwise2_hetero_gen_Prop (t1 t2 : flat_type)
-            : interp_flat_type interp_base_type1 t1 -> interp_flat_type interp_base_type2 t2 -> P
-            := match t1, t2 with
-               | Tbase t1, Tbase t2 => R t1 t2
-               | Unit, Unit => fun _ _ => True
-               | Prod x1 y1, Prod x2 y2
-                 => fun a b => and (interp_flat_type_rel_pointwise2_hetero_gen_Prop x1 x2 (fst a) (fst b))
-                                   (interp_flat_type_rel_pointwise2_hetero_gen_Prop y1 y2 (snd a) (snd b))
-               | Tbase _, _
-               | Unit, _
-               | Prod _ _, _
-                 => fun _ _ => False
-               end.
-        End hetero.
-        Section homogenous.
-          Context (R : forall t, interp_base_type1 t -> interp_base_type2 t -> P).
-
-          Fixpoint interp_flat_type_rel_pointwise2_gen_Prop (t : flat_type)
-            : interp_flat_type interp_base_type1 t -> interp_flat_type interp_base_type2 t -> P
-            := match t with
-               | Tbase t => R t
-               | Unit => fun _ _ => True
-               | Prod x y => fun a b => and (interp_flat_type_rel_pointwise2_gen_Prop x (fst a) (fst b))
-                                            (interp_flat_type_rel_pointwise2_gen_Prop y (snd a) (snd b))
-               end.
-        End homogenous.
-      End gen_prop.
-
-      Definition interp_flat_type_rel_pointwise2_hetero
-        := @interp_flat_type_rel_pointwise2_hetero_gen_Prop Prop and True False.
-      Global Arguments interp_flat_type_rel_pointwise2_hetero _ !_ !_ _ _ / .
-
-      Definition interp_flat_type_rel_pointwise2
-        := @interp_flat_type_rel_pointwise2_gen_Prop Prop and True.
-      Global Arguments interp_flat_type_rel_pointwise2 _ !_ _ _ / .
-
-      Lemma interp_flat_type_rel_pointwise2_hetero_iff {R t} x y
-        : interp_flat_type_rel_pointwise2 (fun t => R t t) t x y
-          <-> interp_flat_type_rel_pointwise2_hetero R t t x y.
-      Proof. induction t; simpl; rewrite_hyp ?*; reflexivity. Qed.
-
-      Section with_coercion.
-        Let Tbase := (@Tbase base_type_code).
-        Local Coercion Tbase : base_type_code >-> flat_type.
-
-        Definition interp_type_rel_pointwise2_hetero R
-          : forall t1 t2, interp_type interp_base_type1 t1
-                          -> interp_type interp_base_type2 t2
-                          -> Prop
-          := interp_type_gen_rel_pointwise2_hetero_hetero _ _ _ _ (interp_flat_type_rel_pointwise2_hetero R) (interp_flat_type_rel_pointwise2_hetero R).
-      End with_coercion.
-      Global Arguments interp_type_rel_pointwise2_hetero _ !_ !_ _ _ / .
-
       Definition interp_type_rel_pointwise2 R
         : forall t, interp_type interp_base_type1 t
                     -> interp_type interp_base_type2 t
                     -> Prop
-        := interp_type_gen_rel_pointwise2 _ _ (interp_flat_type_rel_pointwise2 R).
+        := interp_type_gen_rel_pointwise2 _ _ (interp_flat_type_rel_pointwise R).
       Global Arguments interp_type_rel_pointwise2 _ !_ _ _ / .
-    End flat_type.
-  End rel_pointwise2.
+
+      Definition interp_type_rel_pointwise2_hetero R
+        : forall t1 t2, interp_type interp_base_type1 t1
+                        -> interp_type interp_base_type2 t2
+                        -> Prop
+        := interp_type_gen_rel_pointwise_hetero_hetero _ _ _ _ (fun t1 t2 => interp_flat_type_rel_pointwise_hetero R (Tbase t1) (Tbase t2)) (interp_flat_type_rel_pointwise_hetero R).
+      Global Arguments interp_type_rel_pointwise2_hetero _ !_ !_ _ _ / .
+    End hetero.
+
+    Section homogenous.
+      Context {interp_base_type : base_type_code -> Type}.
+      Definition interp_type_rel_pointwise R
+        := interp_type_gen_rel_pointwise _ (@interp_flat_type_rel_pointwise interp_base_type interp_base_type R).
+    End homogenous.
+  End specialized_type.
 
   Section lifting.
+    Context {interp_base_type1 interp_base_type2 : base_type_code -> Type}.
+    Local Notation interp_flat_type1 := (interp_flat_type interp_base_type1).
+    Local Notation interp_flat_type2 := (interp_flat_type interp_base_type2).
     Let Tbase := (@Tbase base_type_code).
     Local Coercion Tbase : base_type_code >-> flat_type.
 
-    Section flat_type.
-      Context {interp_base_type : base_type_code -> Type}.
-      Local Notation interp_flat_type := (interp_flat_type interp_base_type).
-      Context (R : forall t, interp_flat_type t -> interp_flat_type t -> Prop)
+    Section with_rel.
+      Context (R : forall t, interp_flat_type1 t -> interp_flat_type2 t -> Prop)
               (RUnit : R Unit tt tt).
       Section RProd.
         Context (RProd : forall A B x y, R A (fst x) (fst y) /\ R B (snd x) (snd y) -> R (Prod A B) x y)
                 (RProd' : forall A B x y, R (Prod A B) x y -> R A (fst x) (fst y) /\ R B (snd x) (snd y)).
-        Lemma lift_interp_flat_type_rel_pointwise1 t (x y : interp_flat_type t)
+        Lemma lift_interp_flat_type_rel_pointwise1 t (x : interp_flat_type1 t) (y : interp_flat_type2 t)
           : interp_flat_type_rel_pointwise R t x y -> R t x y.
         Proof. clear RProd'; induction t; simpl; destruct_head_hnf' unit; intuition. Qed.
-        Lemma lift_interp_flat_type_rel_pointwise2 t (x y : interp_flat_type t)
+        Lemma lift_interp_flat_type_rel_pointwise2 t (x : interp_flat_type1 t) (y : interp_flat_type2 t)
           : R t x y -> interp_flat_type_rel_pointwise R t x y.
         Proof. clear RProd; induction t; simpl; destruct_head_hnf' unit; split_and; intuition. Qed.
       End RProd.
       Section RProd_iff.
         Context (RProd : forall A B x y, R A (fst x) (fst y) /\ R B (snd x) (snd y) <-> R (Prod A B) x y).
-        Lemma lift_interp_flat_type_rel_pointwise t (x y : interp_flat_type t)
+        Lemma lift_interp_flat_type_rel_pointwise t (x : interp_flat_type1 t) (y : interp_flat_type2 t)
           : interp_flat_type_rel_pointwise R t x y <-> R t x y.
         Proof.
           split_iff; split; auto using lift_interp_flat_type_rel_pointwise1, lift_interp_flat_type_rel_pointwise2.
         Qed.
       End RProd_iff.
-    End flat_type.
-    Section flat_type2.
-      Context {interp_base_type1 interp_base_type2 : base_type_code -> Type}.
-      Lemma lift_interp_flat_type_rel_pointwise2_f_eq {T} (f g : forall t, _ -> T t) t x y
-        : interp_flat_type_rel_pointwise2
-            interp_base_type1 interp_base_type2
-            (fun t x y => f t x = g t y)
-            t x y
-          <-> SmartVarfMap f x = SmartVarfMap g y.
-      Proof.
-        induction t; unfold SmartVarfMap in *; simpl in *; destruct_head_hnf unit; try tauto.
-        rewrite_hyp !*; intuition congruence.
-      Qed.
-      Lemma lift_interp_flat_type_rel_pointwise2_f_eq_id1 (f : forall t, _ -> _) t x y
-        : interp_flat_type_rel_pointwise2
-            interp_base_type1 interp_base_type2
-            (fun t x y => x = f t y)
-            t x y
-          <-> x = SmartVarfMap f y.
-      Proof. rewrite lift_interp_flat_type_rel_pointwise2_f_eq, SmartVarfMap_id; reflexivity. Qed.
-      Lemma lift_interp_flat_type_rel_pointwise2_f_eq_id2 (f : forall t, _ -> _) t x y
-        : interp_flat_type_rel_pointwise2
-            interp_base_type1 interp_base_type2
-            (fun t x y => f t x = y)
-            t x y
-          <-> SmartVarfMap f x = y.
-      Proof. rewrite lift_interp_flat_type_rel_pointwise2_f_eq, SmartVarfMap_id; reflexivity. Qed.
-    End flat_type2.
+    End with_rel.
+    Lemma lift_interp_flat_type_rel_pointwise_f_eq {T} (f g : forall t, _ -> T t) t x y
+      : @interp_flat_type_rel_pointwise
+          interp_base_type1 interp_base_type2
+          (fun t x y => f t x = g t y)
+          t x y
+        <-> SmartVarfMap f x = SmartVarfMap g y.
+    Proof.
+      induction t; unfold SmartVarfMap in *; simpl in *; destruct_head_hnf unit; try tauto.
+      rewrite_hyp !*; intuition congruence.
+    Qed.
+    Lemma lift_interp_flat_type_rel_pointwise_f_eq_id1 (f : forall t, _ -> _) t x y
+      : @interp_flat_type_rel_pointwise
+          interp_base_type1 interp_base_type2
+          (fun t x y => x = f t y)
+          t x y
+        <-> x = SmartVarfMap f y.
+    Proof. rewrite lift_interp_flat_type_rel_pointwise_f_eq, SmartVarfMap_id; reflexivity. Qed.
+    Lemma lift_interp_flat_type_rel_pointwise_f_eq_id2 (f : forall t, _ -> _) t x y
+      : @interp_flat_type_rel_pointwise
+          interp_base_type1 interp_base_type2
+          (fun t x y => f t x = y)
+          t x y
+        <-> SmartVarfMap f x = y.
+    Proof. rewrite lift_interp_flat_type_rel_pointwise_f_eq, SmartVarfMap_id; reflexivity. Qed.
   End lifting.
 
   Local Ltac t :=
@@ -265,17 +279,17 @@ Section language.
            | _ => solve [ eauto ]
            end.
 
-  Lemma interp_flat_type_rel_pointwise2_flatten_binding_list
+  Lemma interp_flat_type_rel_pointwise_flatten_binding_list
         {interp_base_type1 interp_base_type2 t T} R' e1 e2 v1 v2
         (H : List.In (existT _ t (v1, v2)%core) (flatten_binding_list e1 e2))
-        (HR : interp_flat_type_rel_pointwise2 interp_base_type1 interp_base_type2 R' T e1 e2)
+        (HR : @interp_flat_type_rel_pointwise interp_base_type1 interp_base_type2 R' T e1 e2)
     : R' t v1 v2.
   Proof. induction T; t. Qed.
 
-  Lemma interp_flat_type_rel_pointwise2_hetero_flatten_binding_list2
+  Lemma interp_flat_type_rel_pointwise_hetero_flatten_binding_list2
         {interp_base_type1 interp_base_type2 t1 t2 T1 T2} R' e1 e2 v1 v2
         (H : List.In (existT _ (t1, t2)%core (v1, v2)%core) (flatten_binding_list2 e1 e2))
-        (HR : interp_flat_type_rel_pointwise2_hetero interp_base_type1 interp_base_type2 R' T1 T2 e1 e2)
+        (HR : @interp_flat_type_rel_pointwise_hetero interp_base_type1 interp_base_type2 R' T1 T2 e1 e2)
     : R' t1 t2 v1 v2.
   Proof.
     revert dependent T2; induction T1, T2; t.
@@ -284,15 +298,13 @@ End language.
 
 Global Arguments interp_type_rel_pointwise2 {_ _ _} R {t} _ _.
 Global Arguments interp_type_rel_pointwise2_hetero {_ _ _} R {t1 t2} _ _.
-Global Arguments interp_type_gen_rel_pointwise2_hetero_hetero {_ _ _ _ _} Rsrc Rdst {t1 t2} _ _.
-Global Arguments interp_type_gen_rel_pointwise2_hetero {_ _ _ _ _} Rsrc Rdst {t} _ _.
+Global Arguments interp_type_gen_rel_pointwise_hetero_hetero {_ _ _ _ _} Rsrc Rdst {t1 t2} _ _.
+Global Arguments interp_type_gen_rel_pointwise_hetero {_ _ _ _ _} Rsrc Rdst {t} _ _.
 Global Arguments interp_type_gen_rel_pointwise2 {_ _ _} R {t} _ _.
-Global Arguments interp_flat_type_rel_pointwise2_gen_Prop {_ _ _ P} and True R {t} _ _.
-Global Arguments interp_flat_type_rel_pointwise2_hetero_gen_Prop {_ _ _ P} and True False R {t1 t2} _ _.
-Global Arguments interp_flat_type_rel_pointwise2_hetero {_ _ _} R {t1 t2} _ _.
-Global Arguments interp_flat_type_rel_pointwise0 {_ _} R {t} _.
-Global Arguments interp_flat_type_rel_pointwise2 {_ _ _} R {t} _ _.
-Global Arguments interp_flat_type_rel_pointwise {_} _ _ {_} _ _.
+Global Arguments interp_flat_type_rel_pointwise_gen_Prop {_ _ _ P} and True R {t} _ _.
+Global Arguments interp_flat_type_rel_pointwise_hetero_gen_Prop {_ _ _ P} and True False R {t1 t2} _ _.
+Global Arguments interp_flat_type_rel_pointwise_hetero {_ _ _} R {t1 t2} _ _.
+Global Arguments interp_flat_type_rel_pointwise1 {_ _} R {t} _.
+Global Arguments interp_flat_type_rel_pointwise {_ _ _} R {t} _ _.
 Global Arguments interp_type_rel_pointwise {_} _ _ {_} _ _.
 Global Arguments interp_type_gen_rel_pointwise {_ _} _ {_} _ _.
-Global Arguments interp_flat_type_rel_pointwise {_} _ _ {_} _ _.
