src/SpecificGen/GF5211_32Reflective/Common.v
@@ -509,7 +509,7 @@ Ltac t_correct_and_bounded ropZ_sig Hbounds H0 H1 args :=
   repeat match goal with x := _ |- _ => subst x end;
   cbv [id
          binop_args_to_bounded unop_args_to_bounded unopWireToFE_args_to_bounded op9_args_to_bounded
-         Relations.proj_eq_rel interp_flat_type_rel_pointwise2 SmartVarfMap interp_flat_type smart_interp_flat_map Application.all_binders_for fst snd BoundedWordW.to_wordW' BoundedWordW.boundedWordToWordW BoundedWord.value Application.ApplyInterpedAll Application.ApplyInterpedAll' Application.interp_all_binders_for_of' Application.interp_all_binders_for_to' Application.fst_binder Application.snd_binder interp_flat_type_rel_pointwise2_gen_Prop Relations.related_wordW_boundsi' Relations.related'_wordW_bounds Bounds.upper Bounds.lower Application.remove_all_binders WordW.to_Z] in Hbounds_left, Hbounds_right;
+         Relations.proj_eq_rel interp_flat_type_rel_pointwise SmartVarfMap interp_flat_type smart_interp_flat_map Application.all_binders_for fst snd BoundedWordW.to_wordW' BoundedWordW.boundedWordToWordW BoundedWord.value Application.ApplyInterpedAll Application.ApplyInterpedAll' Application.interp_all_binders_for_of' Application.interp_all_binders_for_to' Application.fst_binder Application.snd_binder interp_flat_type_rel_pointwise_gen_Prop Relations.related_wordW_boundsi' Relations.related'_wordW_bounds Bounds.upper Bounds.lower Application.remove_all_binders WordW.to_Z] in Hbounds_left, Hbounds_right;
   lazymatch goal with
   | [ |- fe5211_32WToZ ?x = _ /\ _ ]
     => generalize dependent x; intros
